theory/JITFlattern.thy
@@ -71,8 +71,6 @@ lemma match_state1_prop:
         done
       done
     done
-      subgoal for x131 x132 apply(cases "eval_testcond x131 xrs",simp_all)
-        done
       subgoal for x151 x152 x153
         apply(unfold exec_store_def,simp_all)
         apply(cases "storev x153 xm1 (Vlong (eval_addrmode64 x151 xrs)) (Vlong (xrs (IR x152)))",simp_all)
@@ -166,405 +164,6 @@ lemma match_state1_prop:
           done
 
 
-(*
-lemma one_step_equiv_layer1:
-  assumes a0:"flat_bpf_sem 1 (l_bin,l_pc,l_jump) (pc, fxst) = fxst'" and
-   a1:"jitflat_bpf lt init_second_layer = (l_bin,l_pc,l_jump)" and
-   a2:"perir_sem 1 lt (pc,xxst) = xxst'" and
-   a3:"xxst = Next xpc xrs xm xss" and
-   a4:"lt \<noteq> []" and
-   a5:"JITFlattern_def.match_state (pc, xxst) (pc, fxst)" and
-   a6:"snd xxst' \<noteq> Stuck" and
-   a7:"unat pc < length lt \<and> unat pc \<ge> 0" and 
-   a8:"well_formed_prog lt" and
-   a9:"snd fxst' \<noteq> Stuck" and
-   a10:"jitper insns = Some lt "
-  shows"JITFlattern_def.match_state xxst' fxst'"
-proof-
-  have "\<exists> xpc1. fxst = Next xpc1 xrs xm xss" using a3 a5 
-    apply(unfold JITFlattern_def.match_state_def match_state1_def) 
-    apply(cases fxst,simp_all)
-    done
-  then obtain xpc1 where a11:"fxst = Next xpc1 xrs xm xss" by auto
-
-  let "?curr_ins" = "lt!(unat pc)"
-  let "?num" = "fst (lt!(unat pc))"
-  let "?off" = "fst (snd (lt!(unat pc)))"
-  let "?l" = "snd (snd (lt!(unat pc)))"
-  (*have "\<exists> num off l. (num, off, l) = lt!(unat pc)" using a4 a7 by (metis prod.exhaust_sel) 
-  then obtain num off l where b0_0:"(num, off, l) = lt!(unat pc)" by auto*)
-  have b0:"(?num, ?off, ?l) = lt!(unat pc)" by simp
- 
-  let "?xpc" = "fst (l_pc ! (unat pc))"
-  have c0:"list_in_list ?l (nat ?xpc) l_bin" 
-    using flattern_l_bin0 init_second_layer_def a1 b0 a4 a7 a8 by metis
-  let "?prefix" = "take (unat pc) lt"
-  let "?suffix" = "drop (unat pc+1) lt"
-  have "?prefix@[(?num,?off,?l)]@?suffix= lt" using append_take_drop_id init_second_layer_def
-    by (simp add: Cons_nth_drop_Suc a7) 
-  hence "?prefix@((?num,?off,?l)#?suffix)= lt" by simp
-
-
-  have "fxst' = flat_bpf_one_step (l_bin,l_pc,l_jump) (pc, Next xpc1 xrs xm xss)" using a0 a11
-    by (metis One_nat_def flat_bpf_sem.simps(1) flat_bpf_sem.simps(2) old.prod.exhaust) 
-  hence c2:"fxst' = (
-  if unat pc \<ge> length l_pc \<or> unat pc < 0 then (pc,Stuck) else 
-  let num = snd (l_pc!(unat pc)) in 
-  let old_xpc = nat (fst (l_pc!(unat pc))) in 
-        if xpc1 \<noteq> old_xpc then (pc, Stuck) else 
-        case x64_decode xpc1 l_bin of Some(_, Pcall_i _) \<Rightarrow>
-         (case find_target_pc_in_l_pc l_jump (uint pc) of 
-              None \<Rightarrow> (pc, Stuck) |
-              Some npc \<Rightarrow> 
-                (let caller = save_x64_caller xrs; fp = save_x64_frame_pointer xrs; 
-                    rs' = upate_x64_stack_pointer xrs (stack_pointer xss) in
-                let ss' = update_stack caller fp (pc+1) xss in
-                  (case ss' of None \<Rightarrow> (pc, Stuck) | 
-                  Some ra \<Rightarrow> (npc, (Next (nat (fst (l_pc!(unat npc)))) rs' xm ra)))))|
-        Some(_, Pcmpq_rr src dst) \<Rightarrow> \<comment>\<open> TODO: if the first byte is the opcode of cmp? \<close>
-          \<comment>\<open> case: BPF JMP \<close>
-          (case x64_sem num l_bin (Next xpc1 xrs xm xss) of
-          Stuck \<Rightarrow> (pc, Stuck) | \<comment>\<open> if one step error, stop, it should be impossible \<close>
-          Next xpc1 rs1 m1 ss1 \<Rightarrow> (
-            if rs1 (CR ZF) = 1 then \<comment>\<open> must JUMP \<close>
-              (case find_target_pc_in_l_pc l_jump (uint pc) of
-              None \<Rightarrow> (pc, Stuck) |
-              Some npc \<Rightarrow>
-                (npc, (Next (nat (fst (l_pc!(unat npc)))) rs1 m1 ss1))) \<comment>\<open> go to the target address in the jited x64 binary \<close>
-            else \<comment>\<open> donot JUMP \<close>
-              (pc+1, Next xpc1 rs1 m1 ss1)
-          ))|
-       Some(_,Pret) \<Rightarrow>
-          let (pc', ss', caller,fp) = update_stack2 xss in 
-          let rs' = restore_x64_caller xrs caller fp in (pc', Next xpc1 rs' xm ss')
-          \<comment>\<open> case: NOT BPF JMP \<close>
-          \<comment>\<open> case: NOT BPF JMP \<close>|
-       _  \<Rightarrow>
-          (pc+1, x64_sem num l_bin (Next xpc1 xrs xm xss)))" 
-    apply(unfold flat_bpf_one_step_def Let_def) 
-    using a3 a11 apply(cases "Next xpc1 xrs xm xss",simp_all)
-    subgoal for x11 by force
-    done
-
-  have c1:"nat ?xpc= xpc1" using a8 c2 a9 by (smt (verit, ccfv_SIG) snd_conv) 
-
-  have "xxst' = perir_step lt (pc,xxst)" using a2 by (metis One_nat_def perir_sem.simps(1) perir_sem.simps(2) split_pairs)
-
-  hence b1:"xxst' = (let (num,off,l) = lt!(unat pc) in 
-       case x64_decode 0 l of
-      Some(_,Pret) \<Rightarrow>
-          (let (pc', ss', caller,fp) = update_stack2 xss in 
-          let rs' = restore_x64_caller xrs caller fp in (pc', Next xpc rs' xm ss'))|
-      Some(_, Pcall_i _) \<Rightarrow>
-        (let caller = save_x64_caller xrs; fp = save_x64_frame_pointer xrs; 
-            rs' = upate_x64_stack_pointer xrs (stack_pointer xss) in
-        let ss' = update_stack caller fp (pc+1) xss in
-          (case ss' of None \<Rightarrow> (pc, Stuck) | 
-          Some ra \<Rightarrow> (off, Next xpc rs' xm ra)))|
-      Some(_, Pcmpq_rr src dst) \<Rightarrow>
-        (let xst_temp = Next 0 xrs xm xss; xst' = x64_sem num l xst_temp in
-          case xst' of
-          Next xpc' rs' m' ss'\<Rightarrow>
-            if rs' (CR ZF) = 1 then (off+pc, xst')
-            else (pc+1, xst') |
-          Stuck \<Rightarrow> (pc, Stuck))|      
-      _ \<Rightarrow>
-        let xst_temp = Next 0 xrs xm xss; xst' = x64_sem num l xst_temp in
-          (pc+1, xst'))" using perir_step_def b0 a2 a3 apply(cases xxst,simp_all)
-    done
-
-  thus ?thesis
-  proof(cases "\<exists> num. x64_decode 0 ?l = Some(num,Pret)")
-    case True
-    have b3:"xxst' = (let (pc', ss', caller,fp) = update_stack2 xss in 
-          let rs' = restore_x64_caller xrs caller fp in (pc', Next xpc rs' xm ss'))"
-      using b1 True b0 apply(cases "x64_decode (0::nat) ?l",simp_all)
-      subgoal for a apply(cases "lt ! unat pc",simp_all)
-        subgoal for aa b c 
-          apply(cases a,simp_all)
-          done
-        done
-      done
-   have b2_1:"?l \<noteq> []"  using a8 apply(unfold well_formed_prog_def) using b0 a4 a7 by blast
-   have "?num >0 " using a8 apply(unfold well_formed_prog_def) using b0 a4 a7 by blast 
-   hence b2_2:"x64_decode 0 ?l \<noteq> None"  apply(cases "x64_decode 0 ?l",simp_all) using True by force
-   hence b2_3:"x64_decode 0 ?l = x64_decode xpc1 l_bin" using b2_2 list_in_list_x64_decode by (metis True add.right_neutral c0 c1) 
-   hence b2_4:"\<exists> num. x64_decode xpc1 l_bin = Some(num,Pret)" using b2_3 True by auto
-   have b2:"fxst' =  (let (pc', ss', caller,fp) = update_stack2 xss in
-          let rs' = restore_x64_caller xrs caller fp in (pc', Next xpc1 rs' xm ss'))" using b2_4 c2 a9 a7
-     apply(cases "x64_decode xpc1 l_bin",simp_all)
-     subgoal for a
-       apply(split if_splits,simp_all)
-       subgoal for num
-         apply(unfold Let_def,simp_all)
-         apply(split if_splits,simp_all)
-         done
-       done
-     done
-    
-   have "JITFlattern_def.match_state xxst' fxst'" 
-     using  a6 a9 b2 b3 by(unfold JITFlattern_def.match_state_def match_state1_def Let_def update_stack2_def,simp_all) 
-    then show ?thesis by simp
-  next
-    case False
-    have b2:"\<not>(\<exists> num. x64_decode 0 ?l = Some(num,Pret))" using False by simp
-    then show ?thesis   
-    proof(cases "(\<exists> d num. x64_decode 0 ?l = Some(num, Pcall_i d))")
-      case True
-      have b3:"(\<exists> d num. x64_decode 0 ?l = Some(num, Pcall_i d))" using True by simp
-      have b4:"xxst' = (let caller = save_x64_caller xrs; fp = save_x64_frame_pointer xrs; 
-            rs' = upate_x64_stack_pointer xrs (stack_pointer xss) in
-        let ss' = update_stack caller fp (pc+1) xss in
-          (case ss' of None \<Rightarrow> (pc, Stuck) | 
-          Some ra \<Rightarrow> (?off, Next xpc rs' xm ra)))" 
-        using True b1 b0 b2 apply(cases "x64_decode 0 ?l",simp_all)
-        subgoal for a
-          apply(cases "lt ! unat pc",simp_all)
-          subgoal for aa b c
-            apply(cases a,simp_all)
-            subgoal for ab ba apply(cases ba,simp_all)
-              subgoal for x21a
-                by (metis fst_conv snd_conv) 
-              done
-            done
-          done
-        done
-              
-      have b2_1:"?l \<noteq> []"  using a8 apply(unfold well_formed_prog_def) using b0 a4 a7 by blast
-      have "?num >0 " using a8 apply(unfold well_formed_prog_def) using b0 a4 a7 by blast 
-      hence b2_2:"x64_decode 0 ?l \<noteq> None" apply(cases "x64_decode 0 ?l",simp_all) using b3 by force 
-
-      
-      (*hence "\<forall> n. \<not> (x64_bin_is_sequential n ?l 0)" using x64_bin_is_sequential_x64_decode_pcall_false by blast*)
-      have d3_1:"x64_decode 0 ?l = x64_decode xpc1 l_bin " 
-        using list_in_list_x64_decode c0 by (metis add.right_neutral c1 b3) 
-      hence d3:"fxst' = (case find_target_pc_in_l_pc l_jump (uint pc) of 
-              None \<Rightarrow> (pc, Stuck) |
-              Some npc \<Rightarrow> 
-                (let caller = save_x64_caller xrs; fp = save_x64_frame_pointer xrs; 
-                    rs' = upate_x64_stack_pointer xrs (stack_pointer xss) in
-                let ss' = update_stack caller fp (pc+1) xss in
-                  (case ss' of None \<Rightarrow> (pc, Stuck) | 
-                  Some ra \<Rightarrow> (npc, (Next (nat (fst (l_pc!(unat npc)))) rs' xm ra)))))"
-        using c2 a1 a7 a9 b0 b3 flattern_num split_pairs 
-        apply(split if_splits,simp_all) (*by (smt (verit))*) 
-        subgoal for d num
-          apply(unfold Let_def,simp_all)
-          apply(split if_splits,simp_all)
-          done
-        done
-  
-      thus ?thesis
-        proof(cases "find_target_pc_in_l_pc l_jump (uint pc) \<noteq> None")
-          case True
-          have "\<exists> npc. find_target_pc_in_l_pc l_jump (uint pc) = Some npc" using True by simp
-          then obtain npc where d5_1:"find_target_pc_in_l_pc l_jump (uint pc) = Some npc" by auto
-          have d5_2:"distinct (map fst [])" by simp
-          have d5_4:"is_increase_list [] []" using is_increase_list_empty by blast 
-          hence d5:"npc = ?off" using a1 b0 d5_2 init_second_layer_def a7 b3 d5_4 d5_1 flattern_jump_index_2
-            by (smt (verit, ccfv_threshold) int_ops(1) list.size(3)) 
-
-          have d6_0:"fxst' = (let caller = save_x64_caller xrs; fp = save_x64_frame_pointer xrs; 
-                    rs' = upate_x64_stack_pointer xrs (stack_pointer xss) in
-                let ss' = update_stack caller fp (pc+1) xss in
-                  (case ss' of None \<Rightarrow> (pc, Stuck) | 
-                  Some ra \<Rightarrow> (?off, (Next (nat (fst (l_pc!(unat ?off)))) rs' xm ra))))" using d5 d3 d5_1 by auto
-          hence d6: "JITFlattern_def.match_state xxst' fxst'" 
-            using b4 d5 d3 True JITFlattern_def.match_state_def match_state1_def a9 a6
-            by (smt (z3) case_prod_beta' option.case_eq_if outcome.simps(4) prod.collapse prod.inject) 
-          then show ?thesis by simp             
-        next
-          case False
-          have "find_target_pc_in_l_pc l_jump (uint pc) = None" using False by simp
-           hence "fxst' = (pc,Stuck)" using d3 by simp
-          then show ?thesis using a9 by auto
-        qed
-    next
-      case False
-      have b5:"(\<not> (\<exists> num. x64_decode 0 ?l = Some(num,Pret))) \<and> (\<not>(\<exists> num d. x64_decode 0 ?l = Some(num, Pcall_i d)))" using False b2 by simp
-      hence bn_1:"?l \<noteq> []" using a8 apply(unfold well_formed_prog_def) using b0 a4 a7 by blast
-      have bn_2:"?num >0 " using a8 apply(unfold well_formed_prog_def) using b0 a4 a7 by blast 
-
-      have c3_0:"list_in_list ?l xpc1 l_bin" using c0 c1 by simp         
-      have c3:"l_bin!xpc1 = ?l!0" using c3_0 bn_1 by (metis list.collapse list_in_list.simps(2) nth_Cons_0)
-      then show ?thesis      
-      proof(cases "(\<exists> num src dst. x64_decode 0 ?l = Some(num, Pcmpq_rr src dst))")
-        
-        case True
-        
-        hence d0:"xxst' = (let xst_temp = Next 0 xrs xm xss; xst' = x64_sem ?num ?l xst_temp in
-          case xst' of
-          Next xpc' rs' m' ss'\<Rightarrow>
-            if rs' (CR ZF) = 1 then (?off+pc, xst')
-            else (pc+1, xst') |
-          Stuck \<Rightarrow> (pc, Stuck) )" using True b1 b0 b5 apply(cases "x64_decode 0 ?l",simp_all)
-        subgoal for a
-          apply(cases "lt ! unat pc",simp_all)
-          subgoal for aa b c
-            apply(cases a,simp_all)
-            subgoal for ab ba apply(cases ba,simp_all)
-              subgoal for x21a
-                by (metis fst_conv snd_conv) 
-              done
-            done
-          done
-        done
-        
-        have d1_1:"\<exists> num src dst. x64_decode xpc1 l_bin = Some(num, Pcmpq_rr src dst)" 
-          using list_in_list_x64_decode c3_0 True by fastforce 
-        hence d1:"fxst' = (case x64_sem (snd (l_pc!(unat pc))) l_bin (Next xpc1 xrs xm xss) of
-          Stuck \<Rightarrow> (pc, Stuck) | \<comment>\<open> if one step error, stop, it should be impossible \<close>
-          Next xpc1 rs1 m1 ss1 \<Rightarrow> (
-            if rs1 (CR ZF) = 1 then \<comment>\<open> must JUMP \<close>
-              (case find_target_pc_in_l_pc l_jump (uint pc) of
-              None \<Rightarrow> (pc, Stuck) |
-              Some npc \<Rightarrow>
-                (npc, (Next (nat (fst (l_pc!(unat npc)))) rs1 m1 ss1))) \<comment>\<open> go to the target address in the jited x64 binary \<close>
-            else \<comment>\<open> donot JUMP \<close>
-              (pc+1, Next xpc1 rs1 m1 ss1)
-          )) " using True a0 c2 a7 a9 c1 by auto 
-        
-        have d4:"(snd (l_pc!(unat pc))) = ?num"
-            by (metis (mono_tags, lifting) a1 a7 b0 flattern_num)         
-        have "\<exists> fxst1. fxst1 = x64_sem ?num l_bin (Next xpc1 xrs xm xss)" by fastforce
-        then obtain fxst1 where d2_0:"fxst1 = x64_sem ?num l_bin (Next xpc1 xrs xm xss)" by auto
-        have "\<exists> xxst1. xxst1 = x64_sem ?num ?l (Next 0 xrs xm xss)" by fastforce
-        then obtain xxst1 where d2_1:"xxst1 = x64_sem ?num ?l (Next 0 xrs xm xss)" by auto
-        have d2_5_1:"xxst1 \<noteq> Stuck" using a6 d1 d2_1 d4 d0 by force
-        hence d2_5:"x64_decode 0 ?l \<noteq> None" using d2_1 apply(cases "x64_decode 0 ?l",simp_all)
-          by (metis (no_types, lifting) Suc_diff_1 bn_2 option.simps(4) x64_sem.simps(3)) 
-
-        have b7_0:"\<exists> num src dst. x64_decode 0 ?l = Some(num, Pcmpq_rr src dst)" using True bn_1 d2_5 by simp
-        have b7:"?num = 1" using a10 b7_0 by (metis a7 b0 jit_prog_prop4)  
-        hence d2_2:"fxst1 = (case x64_decode xpc1 l_bin of
-          None \<Rightarrow> Stuck |
-          Some (sz, ins) \<Rightarrow>
-            x64_sem 0 l_bin (exec_instr ins sz xpc1 xrs xm xss)
-          )" using d2_0 by simp
-        have d2_3_1:"fxst1 \<noteq> Stuck" using a9 d1 d2_0 b0 d4 by auto
-        hence d2_3:"x64_decode xpc1 l_bin \<noteq> None" using d2_2 by(cases "x64_decode xpc1 l_bin",simp_all)
-        hence d2_4:"fxst1 = (case x64_decode xpc1 l_bin of Some (sz, ins) \<Rightarrow> (exec_instr ins sz xpc1 xrs xm xss))" 
-          using d2_2 by force
-
-      
-        have d2_6:"xxst1 = (case x64_decode 0 ?l of Some (sz, ins) \<Rightarrow> (exec_instr ins sz 0 xrs xm xss))"
-          using b7 d2_1 d2_5 by force 
-        
-        have d2_7:"x64_decode 0 ?l = x64_decode xpc1 l_bin" using list_in_list_x64_decode d2_3 d2_5 c3_0 by fastforce 
-        have "\<exists> sz ins. x64_decode 0 ?l = Some (sz, ins)" using d2_5 by simp
-        then obtain sz ins where "x64_decode 0 ?l = Some (sz, ins)" by auto
-        hence d2_8:"xxst1 = (exec_instr ins sz 0 xrs xm xss)" using d2_6 by simp
-        hence d2_9:"fxst1 =(exec_instr ins sz xpc1 xrs xm xss)" using d2_0 d2_1 d2_6 d2_4 d2_7
-          by (metis \<open>x64_decode (0::nat) (snd (snd ((lt::(nat \<times> 64 word \<times> 8 word list) list) ! unat (pc::64 word)))) = Some (sz::nat, ins::instruction)\<close> case_prod_conv option.simps(5)) 
-        have d2:"match_state1 fxst1 xxst1" using match_state1_prop d2_3_1 d2_5_1 d2_8 d2_9 by blast
-          
-          have d3:"\<exists> xpc' xrs1 xm1 xss1. Next xpc' xrs1 xm1 xss1 = fxst1" 
-            using d2 match_state1_def by (smt (verit, ccfv_threshold) outcome.exhaust outcome.simps(5)) 
-          then obtain xpc' xrs1 xm1 xss1 where d4_0:"Next xpc' xrs1 xm1 xss1 = fxst1" by auto
-          have "\<exists> xpc''. Next xpc'' xrs1 xm1 xss1 = xxst1" 
-            using d3 match_state1_def d4_0 by (smt (verit, ccfv_SIG) d2 outcome.exhaust outcome.simps(4) outcome.simps(5))
-          then obtain xpc'' where d4_1:"Next xpc'' xrs1 xm1 xss1 = xxst1" by auto
-          
-          thus ?thesis
-          proof(cases "xrs1 (CR ZF) = 1")
-            case True
-            have d5_0: "xrs1 (CR ZF) = 1" using True by auto
-            thus ?thesis
-            proof(cases "find_target_pc_in_l_pc l_jump (uint pc) \<noteq> None")
-              case True
-                have "\<exists> npc. find_target_pc_in_l_pc l_jump (uint pc) = Some npc" using True by simp
-                then obtain npc where d5_1:"find_target_pc_in_l_pc l_jump (uint pc) = Some npc" by auto
-                have d5_2:"distinct (map fst [])" by simp
-                have d5_4:"is_increase_list [] []" using is_increase_list_empty by blast 
-                hence d5:"npc = ?off+pc" using a1 a4 b0 a7 flattern_jump_index_1 init_second_layer_def d5_2 d5_1 b7_0
-                  by (metis (mono_tags, lifting) Abs_fnat_hom_0 add_0 int_ops(1) list.size(3))
-                                                 
-                have d6_0:"fxst' =  (npc, (Next (nat (fst (l_pc!(unat npc)))) xrs1 xm1 xss1))" 
-                  using d5_0 d5_1 True d4_0 d1 d2_0 d4 by (smt (verit, best) option.simps(5) outcome.simps(4))
-                have d6_1:"xxst' = (?off+pc, xxst1)"
-                  by (smt (verit, ccfv_threshold) d0 d2_1 d4_1 d5_0 outcome.simps(4)) 
-
-                have "JITFlattern_def.match_state fxst' xxst'" 
-                  using d6_0 d6_1 JITFlattern_def.match_state_def d4_1 d5 match_state1_def by auto
-                then show ?thesis using JITFlattern_def.match_state_def d6_0 d6_1 match_state1_def \<open>\<And>thesis::bool. (\<And>xpc''::nat. Next xpc'' (xrs1::preg \<Rightarrow> 64 word) (xm1::nat \<Rightarrow> int \<Rightarrow> 8 word option) (xss1::stack_state) = (xxst1::outcome) \<Longrightarrow> thesis) \<Longrightarrow> thesis\<close> by fastforce 
-               next
-                 case False
-                 have "find_target_pc_in_l_pc l_jump (uint pc) = None" using False by simp
-                 hence "fxst' = (pc,Stuck)" using a9
-                   by (smt (verit, ccfv_SIG) d1 d2_0 d4 d4_0 d5_0 option.case_eq_if outcome.simps(4)) 
-                then show ?thesis using a9 by auto
-              qed
-            next
-              case False
-              have d5_0:"xrs1 (CR ZF) \<noteq> 1" using False by simp
-              have d5_1:"xxst' = (pc+1, xxst1)" by (smt (verit) d0 d2_1 d4_1 d5_0 outcome.simps(4)) 
-              have d5_2:"fxst' = (pc+1, fxst1)" 
-                using d5_0 by (smt (verit, ccfv_threshold) d1 d2_0 d4 d4_0 outcome.simps(4)) 
-            then show ?thesis using d5_1 d5_2 JITFlattern_def.match_state_def d2 d3 d4_1 by force 
-        qed
-
-      next
-        case False
-        have b6:"(\<not>(\<exists> num. x64_decode 0 ?l = Some(num,Pret))) \<and> (\<not>(\<exists> num d. x64_decode 0 ?l = Some(num, Pcall_i d))) \<and> (\<not> (\<exists> num src dst. x64_decode 0 ?l = Some(num, Pcmpq_rr src dst)))" 
-          using b5 False by force 
-          have d0:"xxst' = (let xst_temp = Next 0 xrs xm xss; xst' = x64_sem ?num ?l xst_temp in
-          (pc+1, xst'))" using b6 b0 b1 apply(cases "x64_decode 0 ?l",simp_all)
-            apply(cases "lt ! unat pc",simp_all)
-            subgoal for a apply(cases "lt ! unat pc",simp_all)
-              subgoal for aa b c
-                apply(cases a,simp_all)
-                subgoal for ab ba apply(cases ba,simp_all)
-                  done
-                done
-              done
-            done
-          hence bn_0:"x64_decode 0 ?l \<noteq> None" using d0 a6 bn_2 apply(cases "x64_decode 0 ?l",simp_all)
-            by (smt (verit) Suc_diff_1 option.simps(4) x64_sem.simps(3))
-          hence "x64_decode 0 ?l \<noteq> Some(1,Pret) \<and> (\<forall> d. x64_decode 0 ?l \<noteq> Some(5, Pcall_i d)) \<and> (\<forall> src dst. x64_decode 0 ?l \<noteq> Some(3, Pcmpq_rr src dst))"
-            using  bn_1 b6 by simp
-
-          have "(\<not>(\<exists> num. x64_decode xpc1 l_bin = Some(num,Pret))) \<and> (\<not>(\<exists> num d. x64_decode xpc1 l_bin = Some(num, Pcall_i d))) \<and> (\<not> (\<exists> num src dst. x64_decode xpc1 l_bin = Some(num, Pcmpq_rr src dst)))" 
-            using b6 list_in_list_x64_decode bn_0 c3_0 by fastforce
-          hence c4:"fxst' = (let num = snd (l_pc!(unat pc)) in (pc+1, x64_sem num l_bin (Next xpc1 xrs xm xss)))"
-            using c2 b6  a1 a7 add.right_neutral c1 init_second_layer_def l_pc_length_prop a9 a9 c2 snd_conv
-          apply(cases "x64_decode xpc1 l_bin",simp_all)
-            apply(cases "lt ! unat pc",simp_all)
-            subgoal for a apply(cases "lt ! unat pc",simp_all)
-              subgoal for aa
-                apply(split if_splits,simp_all)
-                done
-              done
-            subgoal for a
-              apply(split if_splits,simp_all)
-                apply(cases a,simp_all)                
-                subgoal for aa b apply(cases b,simp_all)
-                  done
-                done
-              done           
-           
-          have c5_1:"l_pc \<noteq> []"  using a1 a4 apply(unfold init_second_layer_def) using num_corr by fastforce 
-
-          have c5:"fxst' = (pc+1, x64_sem ?num l_bin (Next xpc1 xrs xm xss))"using b0 c5_1 a1 init_second_layer_def c4 a6 a7
-            by (metis (mono_tags, lifting) flattern_num)
-
-          hence c6:"x64_bin_is_sequential (length ?l) ?l 0" using a10 x64_bin_is_sequential_x64_decode2 b6 a7 b0 bn_0 by metis
-          
-          have cn:"match_state1 (snd xxst') (snd fxst')" using c5 d0 c3_0 list_in_list_prop3 c6 a6 a9 by (metis add.right_neutral snd_conv) 
-            
-          have "fst fxst' = pc+1" using c5 by auto
-          moreover have d2:"fst xxst' = pc+1" using d0 by auto
-          hence "fst xxst' = fst fxst'" using calculation by presburger 
-          hence "JITFlattern_def.match_state xxst' fxst'" using cn JITFlattern_def.match_state_def match_state1_def 
-            apply(cases "snd xxst'",simp_all)
-            apply(cases "snd fxst'",simp_all)
-            by (simp add: case_prod_beta')                    
-          then show ?thesis by (simp add: c5 d0) 
-        qed
-      qed
-    qed
-  qed
-*)
-
 lemma one_step_equiv_layer1:
   assumes a0:"flat_bpf_sem 1 (l_bin,l_pc,l_jump) (pc, fxst) = fxst'" and
    a1:"jitflat_bpf lt init_second_layer = (l_bin,l_pc,l_jump)" and
@@ -618,18 +217,18 @@ proof-
                                     Next xpc' rs' m' ss' \<Rightarrow> (npc, (Next xpc' rs' m' ss'))))) |
         Some(sz, Pcmpq_rr src dst) \<Rightarrow> \<comment>\<open> TODO: if the first byte is the opcode of cmp? \<close>
           \<comment>\<open> case: BPF JMP \<close>
-          (case x64_decode (xpc1+sz) l_bin of Some (sz2,Pjcc _ _) \<Rightarrow>
-          (case x64_sem num l_bin (Next xpc1 xrs xm1 xss) of
+          (case x64_decode (xpc1+sz) l_bin of Some (sz2,Pjcc cond _) \<Rightarrow>
+          (if num = 1 then case x64_sem num l_bin (Next xpc1 xrs xm1 xss) of
           Stuck \<Rightarrow> (pc, Stuck) | \<comment>\<open> if one step error, stop, it should be impossible \<close>
           Next xpc1 rs1 m1 ss1 \<Rightarrow> (
           case find_target_pc_in_l_pc l_jump (unat pc) of
                       None \<Rightarrow> (pc, Stuck) |
                       Some npc \<Rightarrow>
-            if rs1 (CR ZF) = 1 then \<comment>\<open> must JUMP \<close>
+            if eval_testcond cond rs1 then \<comment>\<open> must JUMP \<close>
              (npc, (Next (fst (l_pc!(unat npc))) rs1 m1 ss1)) \<comment>\<open> go to the target address in the jited x64 binary \<close>
             else \<comment>\<open> donot JUMP \<close>
               (pc+1, Next (xpc1+sz2) rs1 m1 ss1)
-          ))|
+          )else (pc, Stuck))|
             _ \<Rightarrow> (pc, Stuck)) |
         Some(sz,Pret_anchor) \<Rightarrow>
           (case x64_decode (xpc1+sz) l_bin of Some (sz2,Pret) \<Rightarrow>
@@ -659,13 +258,15 @@ proof-
           let xst_temp = Next sz rs' xm ss' in  
           (case x64_decode sz l of Some(_, Pret) \<Rightarrow> (pc', x64_sem 1 l xst_temp)|
                                                _ \<Rightarrow> (pc,Stuck)))|        
-      Some(_, Pcmpq_rr src dst) \<Rightarrow> 
-        (let xst_temp = Next 0 xrs xm xss; xst' = x64_sem 1 l xst_temp in
-          case xst' of
+       Some(sz, Pcmpq_rr src dst) \<Rightarrow> 
+        (case x64_decode sz l of Some(_, Pjcc cond d ) \<Rightarrow> 
+          let xst_temp = Next 0 xrs xm xss; xst' = x64_sem 1 l xst_temp in
+          (case xst' of
           Next xpc' rs' m' ss'\<Rightarrow>
-            if rs' (CR ZF) = 1 then (off+pc, xst')
+            if eval_testcond cond rs' then (off+pc, xst')
             else (pc+1, xst') |
-          Stuck \<Rightarrow> (pc, Stuck))|      
+          Stuck \<Rightarrow> (pc, Stuck))|
+        _ \<Rightarrow> (pc,Stuck))|      
       _  \<Rightarrow>
         (let xst_temp = Next 0 xrs xm xss; xst' = x64_sem num l xst_temp in
           (pc+1, xst')))" 
@@ -915,72 +516,106 @@ proof-
       proof(cases "(\<exists> num src dst. x64_decode 0 ?l = Some(num, Pcmpq_rr src dst))")
         
         case True
-        
-        hence d0:"xxst' = (let xst_temp = Next 0 xrs xm xss; xst' = x64_sem 1 ?l xst_temp in
-          case xst' of
+        then obtain num src dst where d0_0:"x64_decode 0 ?l = Some(num, Pcmpq_rr src dst)" by auto
+        hence d0:"xxst' = ((case x64_decode num ?l of Some(sz, Pjcc cond d ) \<Rightarrow> 
+          let xst_temp = Next 0 xrs xm xss; xst' = x64_sem 1 ?l xst_temp in
+          (case xst' of
           Next xpc' rs' m' ss'\<Rightarrow>
-            if rs' (CR ZF) = 1 then (?off+pc, xst')
+            if eval_testcond cond rs' then (?off+pc, xst')
             else (pc+1, xst') |
-          Stuck \<Rightarrow> (pc, Stuck) )" using True b1 b0 b5 apply(cases "x64_decode 0 ?l",simp_all)
-        subgoal for a
+          Stuck \<Rightarrow> (pc, Stuck))|
+        _ \<Rightarrow> (pc,Stuck)))" using True b1 b0 b5 apply(cases "x64_decode 0 ?l",simp_all)
           apply(cases "lt ! unat pc",simp_all)
-          subgoal for aa b c
-            apply(cases a,simp_all)
+          subgoal for a b c
+            apply(cases "x64_decode num c ",simp_all)
+            subgoal for aa apply(cases a,simp_all)
+               apply(cases aa,simp_all)
+              subgoal for ab ba apply(cases ba,simp_all)
+                subgoal for x131 x132 apply(unfold Let_def)
+                  apply(cases "exec_instr (Pcmpq_rr src dst) num (0::nat) xrs xm xss",simp_all)             
+              done
+            done
+          subgoal for nat apply(cases aa,simp_all) 
             subgoal for ab ba apply(cases ba,simp_all)
-              subgoal for x21a
-                by (metis fst_conv snd_conv) 
+              subgoal for x131 x132 apply(unfold Let_def)
+                apply(cases "exec_instr (Pcmpq_rr src dst) num (0::nat) xrs xm xss",simp_all)       
+                done
               done
             done
           done
         done
-        
+      done
+      have d0_1:"\<exists> sz2 cond d. x64_decode num ?l = Some (sz2,Pjcc cond d)" 
+      proof(rule ccontr)
+        assume assm:"\<not>(\<exists> sz2 cond d. x64_decode num ?l = Some (sz2,Pjcc cond d))"
+        then obtain sz2 cond d where "\<not>(x64_decode num ?l = Some (sz2,Pjcc cond d))" by auto
+        hence "x64_decode num ?l \<noteq> Some (sz2,Pjcc cond d)" by auto
+        hence "xxst' = (pc,Stuck)" using d0 using assm apply(cases "x64_decode num ?l",simp_all)
+          subgoal for a apply(cases a,simp_all)
+            subgoal for aa b apply(cases b,simp_all)
+              done
+            done
+          done
+        thus "False" using a6 by simp
+      qed
+      then obtain sz2 cond d where d0_2:"x64_decode num ?l = Some (sz2,Pjcc cond d)" by auto
+      hence d0_3:"xxst' = (let xst_temp = Next 0 xrs xm xss; xst' = x64_sem 1 ?l xst_temp in
+          (case xst' of
+          Next xpc' rs' m' ss'\<Rightarrow>
+            if eval_testcond cond rs' then (?off+pc, xst')
+            else (pc+1, xst') |
+          Stuck \<Rightarrow> (pc, Stuck)))" using d0_2 d0 by(cases "x64_decode num ?l",simp_all)
+      have "\<exists> xxst1. xxst1 = x64_sem 1 ?l (Next 0 xrs xm xss)" by fastforce
+      then obtain xxst1 where d2_1:"xxst1 = x64_sem 1 ?l (Next 0 xrs xm xss)" by auto
+      have d2_5_1:"xxst1 \<noteq> Stuck" 
+       proof(rule ccontr)  
+         assume assm:"\<not>(xxst1 \<noteq> Stuck)" 
+         hence "xxst' = (pc,Stuck)" using a6 d0_3 d2_1 by(unfold Let_def,simp_all)
+         thus "False" using a6 by simp
+       qed
+       hence d0_4:"xxst' = (case xxst1 of
+          Next xpc' rs' m' ss'\<Rightarrow>
+            if eval_testcond cond rs' then (?off+pc, xxst1)
+            else (pc+1, xxst1))" using d2_5_1 d2_1 d0_3
+         by (metis (no_types, lifting) outcome.exhaust outcome.simps(4)) 
+       have d2_5:"x64_decode 0 ?l \<noteq> None" using d2_1 d2_5_1 by(cases "x64_decode 0 ?l",simp_all)
+
+
        have d1_1:"\<exists> sz src dst. x64_decode xpc1 l_bin = Some(sz, Pcmpq_rr src dst)" 
           using list_in_list_x64_decode c3_0 True by fastforce 
         then obtain sz src dst where d1_0:"x64_decode xpc1 l_bin = Some(sz, Pcmpq_rr src dst)" by auto
-        hence d1:"fxst' = (case x64_decode (xpc1+sz) l_bin of Some (sz2,Pjcc _ _) \<Rightarrow>
-          (case x64_sem (snd (l_pc!(unat pc))) l_bin (Next xpc1 xrs xm1 xss) of
+        hence d1:"fxst' = (case x64_decode (xpc1+sz) l_bin of Some (sz2,Pjcc cond _) \<Rightarrow>
+          (if (snd (l_pc!(unat pc))) = 1 then case x64_sem (snd (l_pc!(unat pc))) l_bin (Next xpc1 xrs xm1 xss) of
           Stuck \<Rightarrow> (pc, Stuck) | \<comment>\<open> if one step error, stop, it should be impossible \<close>
           Next xpc1 rs1 m1 ss1 \<Rightarrow> (
           case find_target_pc_in_l_pc l_jump (unat pc) of
                       None \<Rightarrow> (pc, Stuck) |
                       Some npc \<Rightarrow>
-            if rs1 (CR ZF) = 1 then \<comment>\<open> must JUMP \<close>
+            if eval_testcond cond rs1 then \<comment>\<open> must JUMP \<close>
              (npc, (Next (fst (l_pc!(unat npc))) rs1 m1 ss1)) \<comment>\<open> go to the target address in the jited x64 binary \<close>
             else \<comment>\<open> donot JUMP \<close>
               (pc+1, Next (xpc1+sz2) rs1 m1 ss1)
-          ))|
-            _ \<Rightarrow> (pc, Stuck))" using True a0 c2 a7 a9 c1 by auto 
-        hence d1_2:"\<exists> sz2 cond d. x64_decode (xpc1+sz) l_bin = Some (sz2,Pjcc cond d)" 
-          using a9 apply(cases "x64_decode (xpc1+sz) l_bin",simp_all)
-          subgoal for a apply(cases a,simp_all)
-            subgoal for aa b by(cases b,simp_all)
-            done
-          done
-        then obtain sz2 cond d where d1_3:"x64_decode (xpc1+sz) l_bin = Some (sz2,Pjcc cond d)" by auto
-        hence d1_4:"fxst' = ((case x64_sem (snd (l_pc!(unat pc))) l_bin (Next xpc1 xrs xm1 xss) of
+          )else (pc, Stuck))|
+            _ \<Rightarrow> (pc, Stuck))" using True a0 c2 a7 a9 c1 apply(split if_splits,simp_all) by(unfold Let_def,simp_all)
+        have d1_3:"x64_decode (xpc1+sz) l_bin = Some (sz2,Pjcc cond d)"
+          by (metis add.right_neutral c3_0 d0_0 d0_2 d1_0 list_in_list_x64_decode old.prod.inject option.inject)
+       have d4:"(snd (l_pc!(unat pc))) = ?num"
+         by (metis (mono_tags, lifting) a1 a7 b0 flattern_num)     
+       have b7:"?num = 1" by (metis a10 a7 b0 d0_0 jit_prog_prop4)    
+       hence d1_4:"fxst' = ((case x64_sem (snd (l_pc!(unat pc))) l_bin (Next xpc1 xrs xm1 xss) of
           Stuck \<Rightarrow> (pc, Stuck) | \<comment>\<open> if one step error, stop, it should be impossible \<close>
           Next xpc1 rs1 m1 ss1 \<Rightarrow> (
           case find_target_pc_in_l_pc l_jump (unat pc) of
                       None \<Rightarrow> (pc, Stuck) |
                       Some npc \<Rightarrow>
-            if rs1 (CR ZF) = 1 then \<comment>\<open> must JUMP \<close>
+            if eval_testcond cond rs1 then \<comment>\<open> must JUMP \<close>
              (npc, (Next (fst (l_pc!(unat npc))) rs1 m1 ss1)) \<comment>\<open> go to the target address in the jited x64 binary \<close>
             else \<comment>\<open> donot JUMP \<close>
               (pc+1, Next (xpc1+sz2) rs1 m1 ss1)
-          )))" using d1 d1_3 by(cases "x64_decode (xpc1+sz) l_bin",simp_all)
-
-        have d4:"(snd (l_pc!(unat pc))) = ?num"
-          by (metis (mono_tags, lifting) a1 a7 b0 flattern_num)      
-        have b7_0:"\<exists> num src dst. x64_decode 0 ?l = Some(num, Pcmpq_rr src dst)" using True bn_1 by simp
-        have b7:"?num = 1" using a10 b7_0 by (metis a7 b0 jit_prog_prop4)  
+          )))" using d1 d1_3 d4 by(cases "x64_decode (xpc1+sz) l_bin",simp_all)
 
         have "\<exists> fxst1. fxst1 = x64_sem 1 l_bin (Next xpc1 xrs xm xss)" by fastforce
-        then obtain fxst1 where d2_0:"fxst1 = x64_sem ?num l_bin (Next xpc1 xrs xm1 xss)" by auto
-        have "\<exists> xxst1. xxst1 = x64_sem ?num ?l (Next 0 xrs xm xss)" by fastforce
-        then obtain xxst1 where d2_1:"xxst1 = x64_sem 1 ?l (Next 0 xrs xm xss)" by auto
-        have d2_5_1:"xxst1 \<noteq> Stuck" using a6 d1 d2_1 d4 d0 by force
-        hence d2_5:"x64_decode 0 ?l \<noteq> None" using d2_1 by(cases "x64_decode 0 ?l",simp_all)
-                
+        then obtain fxst1 where d2_0:"fxst1 = x64_sem ?num l_bin (Next xpc1 xrs xm1 xss)" by auto        
         hence d2_2:"fxst1 = (case x64_decode xpc1 l_bin of
           None \<Rightarrow> Stuck |
           Some (sz, ins) \<Rightarrow>
@@ -1001,17 +636,17 @@ proof-
           by (metis \<open>x64_decode (0::nat) (snd (snd ((lt::(nat \<times> 64 word \<times> 8 word list) list) ! unat (pc::64 word)))) = Some (sz::nat, ins::instruction)\<close> case_prod_conv option.simps(5)) 
         have d2:"match_state1 fxst1 xxst1" using match_state1_prop d2_3_1 d2_5_1 d2_8 d2_9 a11 by blast
           
-          have d3:"\<exists> xpc' xrs1 xm' xss1. Next xpc' xrs1 xm' xss1 = fxst1" 
-            using d2 match_state1_def by (smt (verit, ccfv_threshold) outcome.exhaust outcome.simps(5)) 
-          then obtain xpc' xrs1 xm' xss1 where d4_0:"Next xpc' xrs1 xm' xss1 = fxst1" by auto
-          have "\<exists> xpc'' xm''. Next xpc'' xrs1 xm'' xss1 = xxst1" 
-            using d3 match_state1_def d4_0 by (smt (verit, ccfv_SIG) d2 outcome.exhaust outcome.simps(4) outcome.simps(5))
-          then obtain xpc'' xm'' where d4_1:"Next xpc'' xrs1 xm'' xss1 = xxst1" by auto
-
+        have d3:"\<exists> xpc' xrs1 xm' xss1. Next xpc' xrs1 xm' xss1 = fxst1" 
+          using d2 match_state1_def by (smt (verit, ccfv_threshold) outcome.exhaust outcome.simps(5)) 
+        then obtain xpc' xrs1 xm' xss1 where d4_0:"Next xpc' xrs1 xm' xss1 = fxst1" by auto
+        have "\<exists> xpc'' xm''. Next xpc'' xrs1 xm'' xss1 = xxst1" 
+          using d3 match_state1_def d4_0 by (smt (verit, ccfv_SIG) d2 outcome.exhaust outcome.simps(4) outcome.simps(5))
+        then obtain xpc'' xm'' where d4_1:"Next xpc'' xrs1 xm'' xss1 = xxst1" by auto
+            
         hence d4_2:"fxst' = (case find_target_pc_in_l_pc l_jump (unat pc) of
                       None \<Rightarrow> (pc, Stuck) |
                       Some npc \<Rightarrow>
-            if xrs1 (CR ZF) = 1 then \<comment>\<open> must JUMP \<close>
+              if eval_testcond cond xrs1 then  \<comment>\<open> must JUMP \<close>
              (npc, (Next (fst (l_pc!(unat npc))) xrs1 xm' xss1)) \<comment>\<open> go to the target address in the jited x64 binary \<close>
             else \<comment>\<open> donot JUMP \<close>
               (pc+1, Next (xpc'+sz2) xrs1 xm' xss1))" using d1_4 d4_0 d2_3_1 d2_0 
@@ -1022,16 +657,16 @@ proof-
         then obtain npc where d5_1:"find_target_pc_in_l_pc l_jump (unat pc) = Some npc" by auto
         have d5_2:"distinct (map fst [])" by simp
         have d5_4:"is_increase_list [] []" using is_increase_list_empty by blast 
-        hence d5:"npc = ?off+pc" using a1 a4 b0 a7 flattern_jump_index_1 init_second_layer_def d5_2 d5_1 b7_0
+        hence d5:"npc = ?off+pc" using a1 a4 b0 a7 flattern_jump_index_1 init_second_layer_def d5_2 d5_1 True
         by (metis (mono_tags, lifting) Abs_fnat_hom_0 add_0 list.size(3))        
           thus ?thesis
-          proof(cases "xrs1 (CR ZF) = 1")
+          proof(cases "eval_testcond cond xrs1")
             case True
-            have d5_0: "xrs1 (CR ZF) = 1" using True by auto                                        
+            have d5_0: "eval_testcond cond xrs1" using True by auto                                        
                 have d6_0:"fxst' =  (npc, (Next  (fst (l_pc!(unat npc))) xrs1 xm' xss1))" 
                   using d5_1 d4_2 True by simp
                 have d6_1:"xxst' = (?off+pc, xxst1)"
-                  by (smt (verit, ccfv_threshold) d0 d2_1 d4_1 d5_0 outcome.simps(4))                
+                  using d0_4 d4_1 True by(cases xxst1,simp_all)
                 hence "JITFlattern_def.match_state fxst' xxst'" 
                   using d6_0 d6_1 JITFlattern_def.match_state_def d4_1 d5 match_state1_def d2 d4_0 by force 
                 then show ?thesis using JITFlattern_def.match_state_def d6_0 d6_1 match_state1_def by fastforce 
@@ -1039,8 +674,8 @@ proof-
                 
             next
               case False
-              have d5_0:"\<not> (xrs1 (CR ZF) = 1)" using False by simp
-              have d6_1:"xxst' = (pc+1, xxst1)" by (smt (verit) d0 d2_1 d4_1 d5_0 outcome.simps(4)) 
+              have d5_0:"\<not> (eval_testcond cond xrs1)" using False by simp
+              have d6_1:"xxst' = (pc+1, xxst1)" using d0_4 d4_1 False by force
               have d6_2:"fxst' = (pc+1, Next (xpc'+sz2) xrs1 xm' xss1)" 
                 using d4_2 d5_0 d5_1 by(cases "find_target_pc_in_l_pc l_jump (unat pc)",simp_all)                
             then show ?thesis using JITFlattern_def.match_state_def d4_1 d6_1 fst_conv match_state1_def d2 d4_0 by force 
